coq/NRA/Typing/TNRAInfer.v
@@ -112,20 +112,22 @@ Section TNRAInfer.
 
   Fixpoint infer_nra_type (e:nra) (τin:rtype) : option rtype :=
     match e with
-      | AID => Some τin
-      | AConst d => infer_data_type (normalize_data brand_relation_brands d)
-      | ABinop b op1 op2 =>
+      | NRAGetConstant s =>
+        tdot τconstants s
+      | NRAID => Some τin
+      | NRAConst d => infer_data_type (normalize_data brand_relation_brands d)
+      | NRABinop b op1 op2 =>
         let binf (τ₁ τ₂:rtype) := infer_binary_op_type b τ₁ τ₂ in
         olift2 binf (infer_nra_type op1 τin) (infer_nra_type op2 τin)
-      | AUnop u op1 =>
+      | NRAUnop u op1 =>
         let unf (τ₁:rtype) := infer_unary_op_type u τ₁ in
         olift unf (infer_nra_type op1 τin)
-      | AMap op1 op2 =>
+      | NRAMap op1 op2 =>
         let mapf (τ₁:rtype) :=
             olift (fun x => lift (fun y => Coll y) (infer_nra_type op1 x)) (tuncoll τ₁)
         in
         olift mapf (infer_nra_type op2 τin)
-      | AMapConcat op1 op2 =>
+      | NRAMapProduct op1 op2 =>
         let mapconcatf (τ₁:list (string*rtype)) :=
             match RecMaybe Closed τ₁ with
               | None => None
@@ -137,7 +139,7 @@ Section TNRAInfer.
             end
         in
         olift mapconcatf (olift tmapConcatInput (infer_nra_type op2 τin))
-      | AProduct op1 op2 =>
+      | NRAProduct op1 op2 =>
         let mapconcatf (τ₁:list (string*rtype)) :=
             match RecMaybe Closed τ₁ with
               | None => None
@@ -149,7 +151,7 @@ Section TNRAInfer.
             end
         in
         olift mapconcatf (olift tmapConcatInput (infer_nra_type op1 τin))
-      | ASelect op1 op2 =>
+      | NRASelect op1 op2 =>
         let selectf (τ₁:rtype) :=
             match tuncoll τ₁ with
               | Some τ₁' =>
@@ -165,7 +167,7 @@ Section TNRAInfer.
             end
         in
         olift selectf (infer_nra_type op2 τin)
-      | ADefault op1 op2 =>
+      | NRADefault op1 op2 =>
         match ((infer_nra_type op1 τin), (infer_nra_type op2 τin)) with
             | (Some τ₁', Some τ₂') =>
               match (tuncoll τ₁', tuncoll τ₂') with
@@ -175,7 +177,7 @@ Section TNRAInfer.
               end
             | (_, _) => None
         end
-      | AEither op1 op2 =>
+      | NRAEither op1 op2 =>
         match tuneither τin with
         | Some (τl, τr) =>
           match ((infer_nra_type op1 τl), (infer_nra_type op2 τr)) with
@@ -187,7 +189,7 @@ Section TNRAInfer.
           end
         | _ => None
         end
-      | AEitherConcat op1 op2 =>
+      | NRAEitherConcat op1 op2 =>
         match (infer_nra_type op1 τin, infer_nra_type op2 τin) with
         | (Some τeither, Some τrecplus) =>          
           match tuneither τeither with
@@ -201,11 +203,9 @@ Section TNRAInfer.
           end
         | (_, _) => None
         end
-      | AApp op1 op2 =>
+      | NRAApp op1 op2 =>
         let appf (τ₁:rtype) := infer_nra_type op1 τ₁ in
         olift appf (infer_nra_type op2 τin)
-      | AGetConstant s =>
-        tdot τconstants s
     end.
 
   Lemma infer_nra_type_correct (τin τout:rtype) (e:nra) :
@@ -215,27 +215,29 @@ Section TNRAInfer.
     intros.
     revert τin τout H.
     nra_cases (induction e) Case; intros; simpl in H.
-    - Case "AID"%string.
+    - Case "NRAGetConstant"%string.
+      apply type_NRAGetConstant; assumption.
+    - Case "NRAID"%string.
       inversion H; clear H.
-      apply ATID.
-    - Case "AConst"%string.
-      apply ATConst.
+      apply type_NRAID.
+    - Case "NRAConst"%string.
+      apply type_NRAConst.
       apply infer_data_type_correct. assumption.
-    - Case "ABinop"%string.
+    - Case "NRABinop"%string.
       specialize (IHe1 τin); specialize (IHe2 τin).
       destruct (infer_nra_type e1 τin); destruct (infer_nra_type e2 τin); simpl in *;
       try discriminate.
       specialize (IHe1 r eq_refl); specialize (IHe2 r0 eq_refl).
-      apply (@ATBinop m τconstants τin r r0 τout); try assumption.
+      apply (@type_NRABinop m τconstants τin r r0 τout); try assumption.
       apply infer_binary_op_type_correct; assumption.
-    - Case "AUnop"%string.
+    - Case "NRAUnop"%string.
       specialize (IHe τin).
       destruct (infer_nra_type e τin); simpl in *;
       try discriminate.
       specialize (IHe r eq_refl).
-      apply (@ATUnop m τconstants τin r τout); try assumption.
+      apply (@type_NRAUnop m τconstants τin r τout); try assumption.
       apply infer_unary_op_type_correct; assumption.
-    - Case "AMap"%string.
+    - Case "NRAMap"%string.
       case_eq (infer_nra_type e2 τin); intros; simpl in *.
       + specialize (IHe2 τin r H0). rewrite H0 in H. simpl in *.
         unfold lift in H.
@@ -245,13 +247,13 @@ Section TNRAInfer.
         specialize (IHe1 r0 r1 H).
         rewrite H in H3.
         inversion H3.
-        apply (@ATMap m τconstants τin r0 r1); try assumption.
+        apply (@type_NRAMap m τconstants τin r0 r1); try assumption.
         apply tuncoll_correct in H1.
         rewrite <- H1; assumption.
         rewrite H in H3; congruence.
         rewrite H1 in H; simpl in H; congruence.
       + rewrite H0 in H. simpl in H; congruence.
-    - Case "AMapConcat"%string.
+    - Case "NRAMapProduct"%string.
       case_eq (infer_nra_type e2 τin); intros.
       + specialize (IHe2 τin r H0). rewrite H0 in H; simpl in *.
         unfold tmapConcatInput in H.
@@ -286,8 +288,8 @@ Section TNRAInfer.
             by apply RecMaybe_pf_some.
           simpl in H.
           clear e eq22 H1 eq21 H0.
-          generalize (@ATMapConcat m τconstants τin l1' l2' (rec_concat_sort l1' l2')
-                                   e1 e2 pf1' pf2' H2 IHe1 IHe2 eq_refl); intros.
+          generalize (@type_NRAMapProduct m τconstants τin l1' l2' (rec_concat_sort l1' l2')
+                                          e1 e2 pf1' pf2' H2 IHe1 IHe2 eq_refl); intros.
           assert (τout = (Coll (Rec Closed (rec_concat_sort l1' l2') H2))).
           assert ((@RecMaybe (@basic_model_foreign_type m)
             (@brand_model_relation (@basic_model_foreign_type m)
@@ -321,7 +323,7 @@ Section TNRAInfer.
           assumption.
         * rewrite H0 in H; simpl in H; congruence.
       + rewrite H0 in H; simpl in H; congruence.
-    - Case "AProduct"%string.
+    - Case "NRAProduct"%string.
       case_eq (infer_nra_type e1 τin); intros.
       case_eq (infer_nra_type e2 τin); intros.
       + specialize (IHe1 τin r H0). rewrite H0 in H; simpl in *.
@@ -354,7 +356,7 @@ Section TNRAInfer.
         assert (RecMaybe Closed (rec_concat_sort l1' l2') = Some (Rec Closed (rec_concat_sort l1' l2') H2))
           by apply RecMaybe_pf_some.
         clear e eq22 H1 eq21 srl0 H0.
-        generalize (@ATProduct m τconstants τin l1' l2' (rec_concat_sort l1' l2')
+        generalize (@type_NRAProduct m τconstants τin l1' l2' (rec_concat_sort l1' l2')
                                e1 e2 pf1' pf2' H2 IHe1 IHe2 eq_refl); intros.
         assert (τout = (Coll (Rec Closed (rec_concat_sort l1' l2') H2))).
           assert ((@RecMaybe (@basic_model_foreign_type m)
@@ -392,7 +394,7 @@ Section TNRAInfer.
         destruct (RecMaybe Closed l); congruence.
         congruence.
       + rewrite H0 in H; simpl in H; congruence.
-    - Case "ASelect"%string.
+    - Case "NRASelect"%string.
       simpl.
       case_eq (infer_nra_type e2 τin); intros; simpl in *.
       + specialize (IHe2 τin r H0). rewrite H0 in H. simpl in *.
@@ -405,7 +407,7 @@ Section TNRAInfer.
         destruct r1; try congruence; simpl in *.
         destruct x; try congruence; simpl in *.
         inversion H3; clear H3 H2.
-        apply (@ATSelect m τconstants τin r0); try assumption.
+        apply (@type_NRASelect m τconstants τin r0); try assumption.
         assert (exist (fun τ₀ : rtype₀ => wf_rtype₀ τ₀ = true) Bool₀ e = Bool).
         apply rtype_fequal; reflexivity.
         rewrite H0 in IHe1. assumption.
@@ -414,7 +416,7 @@ Section TNRAInfer.
         rewrite H in H3; congruence.
         rewrite H1 in H; congruence.
       + rewrite H0 in H. simpl in H; congruence.
-    - Case "ADefault"%string.
+    - Case "NRADefault"%string.
       specialize (IHe1 τin); specialize (IHe2 τin).
       destruct (infer_nra_type e1 τin); destruct (infer_nra_type e2 τin); simpl in *;
       try discriminate.
@@ -431,8 +433,8 @@ Section TNRAInfer.
       apply rtype_fequal; simpl; reflexivity.
       elim H; clear H; intros.
       rewrite <- H in *.
-      apply ATDefault; assumption.
-    - Case "AEither"%string.
+      apply type_NRADefault; assumption.
+    - Case "NRAEither"%string.
       unfold tuneither in H.
       destruct τin.
       destruct x; simpl in *; try discriminate.
@@ -444,9 +446,9 @@ Section TNRAInfer.
       specialize (IHe1 _ _ H0).
       specialize (IHe2 _ _ H1).
       erewrite Either_canon
-      ; eapply ATEither
+      ; eapply type_NRAEither
       ; eauto.
-    - Case "AEitherConcat"%string.
+    - Case "NRAEitherConcat"%string.
       case_eq (infer_nra_type e1 τin); case_eq (infer_nra_type e2 τin); simpl in *; intros;
       rewrite H0 in *; rewrite H1 in *; try discriminate.
       unfold tuneither in H.
@@ -489,15 +491,13 @@ Section TNRAInfer.
       rewrite eqq1, eqq2 in IHe1.
       destruct (to_Rec _ _ e0) as [? eqq3].
       rewrite eqq3 in IHe2.
-      eapply ATEitherConcat; eauto.
-    - Case "AApp"%string.
+      eapply type_NRAEitherConcat; eauto.
+    - Case "NRAApp"%string.
       specialize (IHe2 τin).
       destruct (infer_nra_type e2 τin).
       specialize (IHe2 r eq_refl).
       econstructor; eauto.
       simpl in *; congruence.
-    - Case "AGetConstant"%string.
-      apply ATGetConstant; assumption.
   Qed.
 
   (* Still should try and prove most specific and completeness theorems ... *)
