coq/Translation/LambdaNRAtoNRAEnv.v
@@ -36,7 +36,7 @@ Section LambdaNRAtoNRAEnv.
     | LNRABinop b op1 op2 => NRAEnvBinop b (lambda_nra_to_nraenv op1) (lambda_nra_to_nraenv op2)
     | LNRAUnop u op1 => NRAEnvUnop u (lambda_nra_to_nraenv op1)
     | LNRAMap lop1 op2 => NRAEnvMap (nraenv_of_lnra_lambda lop1) (lambda_nra_to_nraenv op2)
-    | LNRAMapConcat lop1 op2 => NRAEnvMapConcat (nraenv_of_lnra_lambda lop1) (lambda_nra_to_nraenv op2)
+    | LNRAMapProduct lop1 op2 => NRAEnvMapProduct (nraenv_of_lnra_lambda lop1) (lambda_nra_to_nraenv op2)
     | LNRAProduct op1 op2 => NRAEnvProduct (lambda_nra_to_nraenv op1) (lambda_nra_to_nraenv op2)
     | LNRAFilter lop1 op2 => NRAEnvSelect (nraenv_of_lnra_lambda lop1) (lambda_nra_to_nraenv op2)
     end
@@ -88,7 +88,7 @@ Section LambdaNRAtoNRAEnv.
   Qed.
 
   Lemma  lambda_nra_to_nraenv_map_concat_eq lop1 op2 :
-    lambda_nra_to_nraenv (LNRAMapConcat lop1 op2) = NRAEnvMapConcat (nraenv_of_lnra_lambda lop1) (lambda_nra_to_nraenv op2).
+    lambda_nra_to_nraenv (LNRAMapProduct lop1 op2) = NRAEnvMapProduct (nraenv_of_lnra_lambda lop1) (lambda_nra_to_nraenv op2).
   Proof.
     reflexivity.
   Qed.
@@ -151,7 +151,7 @@ Section LambdaNRAtoNRAEnv.
       - Case "LNRAMap"%string.
         rewrite (IHq2 d1 d2).
         reflexivity.
-      - Case "LNRAMapConcat"%string.
+      - Case "LNRAMapProduct"%string.
         rewrite (IHq2 d1 d2).
         reflexivity.
       - Case "LNRAProduct"%string.
@@ -195,13 +195,13 @@ Section LambdaNRAtoNRAEnv.
         autorewrite with lambda_nra.
         rewrite (IHq1 _ x).
         reflexivity.
-      - Case "LNRAMapConcat"%string.
+      - Case "LNRAMapProduct"%string.
         rewrite <- (IHq2 _ d).
         apply olift_ext; intros.
         apply lift_oncoll_ext; intros.
         subst.
         f_equal.
-        apply rmap_concat_ext; intros.
+        apply rmap_product_ext; intros.
         autorewrite with lambda_nra.
         rewrite (IHq1 _ x).
         reflexivity.
@@ -257,13 +257,13 @@ Section LambdaNRAtoNRAEnv.
         rewrite IHl1.
         rewrite rec_sort_rec_sort_app1.
         trivial.
-      - Case "LNRAMapConcat"%string.
+      - Case "LNRAMapProduct"%string.
         rewrite <- IHl2.
         apply olift_ext; intros.
         apply lift_oncoll_ext; intros.
         subst.
         f_equal.
-        apply rmap_concat_ext; intros.
+        apply rmap_product_ext; intros.
         rewrite IHl1.
         rewrite rec_sort_rec_sort_app1.
         trivial.
